BB52Theorem.v
@@ -13,11 +13,19 @@ From BusyCoq Require Import Encodings.
 From BusyCoq Require Import CustomTactics.
 From BusyCoq Require Import Decider_Pipeline.
 
+
 From BusyCoq Require Import Decider_Loop.
+From BusyCoq Require Import Decider_Loop_Parameters.
 From BusyCoq Require Import Decider_NGramCPS.
 From BusyCoq Require Import Decider_NGramCPS_Parameters.
+
+From BusyCoq Require Import Decider_Verifier_FAR_Parameters.
 From BusyCoq Require Import Decider_Verifier_FAR_MITM_WDFA_Parameters.
 From BusyCoq Require Import Decider_RepWL_Parameters.
+
+From BusyCoq Require Import Decider_Halt_Parameters.
+
+
 
 From BusyCoq Require Import Sporadic_NonHalt.
 
